biglir.v
@@ -63,31 +63,19 @@ Inductive bigStep : Mem -> IRE -> Mem -> option IRE -> Prop :=
     m'/ e2 ==> m'' / IRENum idx ->
     m''/ e3 ==> fail ->
     m / IRESet e1 e2 e3 ==> fail
-| BStFun : forall m e m' var body,
-    m / e ==> m' / IRELamb var IRTStar body ->
-    m / IREFun e ==> m' / IREFun (IRELamb var IRTStar body)
-| BStFun1F : forall m e,
-    m / e ==> fail ->
-    m / IREFun e ==> fail
-| BStLambapp : forall m e1 m' var t body e2 m'' v2 m''' res,
-     m / e1 ==> m' / IRELamb var t body ->
-     m' / e2 ==> m'' / v2 ->
-     m'' / ([var := v2] body) ==> m''' / res ->
-     m / IRELambApp e1 e2 ==> m''' / res
-| BStLambapp1F : forall m e1 e2,
-     m / e1 ==> fail ->
-     m / IRELambApp e1 e2 ==> fail
-| BStLambapp2F : forall m e1 m' var t body e2,
-     m / e1 ==> m' / IRELamb var t body ->
-     m' / e2 ==> fail ->
-     m / IRELambApp e1 e2 ==> fail
-| BStLambapp3F : forall m e1 m' var t body e2 m'' v2,
-     m / e1 ==> m' / IRELamb var t body ->
-     m' / e2 ==> m'' / v2 ->
-     m'' / ([var := v2] body) ==> fail ->
-     m / IRELambApp e1 e2 ==> fail
+| BStLet : forall m exp m' v1 var t body m'' res,
+     m / exp ==> m' / v1 ->
+     m' / ([var := v1] body) ==> m'' / res ->
+     m / IRELet var t exp body ==> m'' / res
+| BStLet1F : forall m exp var t body,
+     m / exp ==> fail ->
+     m / IRELet var t exp body ==> fail
+| BStLet2F : forall m exp m' v1 var t body,
+     m / exp ==> m' / v1 ->
+     m' / ([var := v1] body) ==> fail ->
+     m / IRELet var t exp body ==> fail
 | BStFunapp : forall m e1 m' var body e2 m'' v2 m''' res,
-    m / e1 ==> m' / IREFun (IRELamb var IRTStar body) ->
+    m / e1 ==> m' / IREFun var body ->
     m' / e2 ==> m'' / v2 ->
     m'' / ([var := v2] body) ==> m''' / res ->
     m / IREFunApp e1 e2 ==> m''' / res
@@ -99,7 +87,7 @@ Inductive bigStep : Mem -> IRE -> Mem -> option IRE -> Prop :=
     m' / e2 ==> fail ->
     m / IREFunApp e1 e2 ==> fail
 | BStFunapp3F : forall m e1 m' var body e2 m'' v2,
-    m / e1 ==> m' / IREFun (IRELamb var IRTStar body) ->
+    m / e1 ==> m' / IREFun var body ->
     m' / e2 ==> m'' / v2 ->
     m'' / ([var := v2] body) ==> fail ->
     m / IREFunApp e1 e2 ==> fail
@@ -159,14 +147,14 @@ Proof.
       HT : _ |= ?E : _,
       IH : mem_correct ?M -> _ -> _ |= ?E : _ -> _ |- _] =>
         specialize (IH HM _ HT _ eq_refl) as [? [? ?]]
-  end;
-  (* handle cases that need substitution *)
+  end
+  (* handle cases that need substitution *
   try match goal with
     | [HT: MEmpty |= IRELamb ?V _ ?B : ETLamb ?T1 ?T2,
        HTV: MEmpty |= ?Arg : (ETn ?T1) |- _] =>
         assert (MEmpty |= [V := Arg] B : T2) by
       (inversion HT; subst; eauto using subst_typing)
-    end
+    end *)
   );
   eauto using IRTyping,Value,mem_correct_fresh,mem_correct_update;
   (* handle substitutions inside FUN (not pretty yet) *)
@@ -175,6 +163,10 @@ Proof.
     eapply IHHst3; eauto).
   - (* use mem_correct for queries *)
     unfold mem_correct in H3. split; eapply H3.
+  - eapply IHHst2; eauto.
+    inversion HTy; subst. eauto using subst_typing.
+  - eapply IHHst2; eauto.
+    inversion HTy; subst. eauto using subst_typing.
   - (* Unboxing step needs an extra inversion on type judgment
        and value to get inside the boxed value *)
     split.
@@ -182,6 +174,39 @@ Proof.
     * inversion H1; trivial.
 Qed.
 
+
+Lemma BstepValue : forall (m m' : Mem) e e' t,
+  m / e ==> m' / e' ->
+  mem_correct m ->
+  MEmpty |= e : t ->
+  Value e'.
+Proof. apply BPreservation. Qed.
+
+
+Lemma BstepTy : forall (m m' : Mem) e e' t,
+  m / e ==> m' / e' ->
+  mem_correct m ->
+  MEmpty |= e : t ->
+  MEmpty |= e' : t.
+Proof. apply BPreservation. Qed.
+
+
+(* Propagate 'mem_correct' to all memories *)
+Ltac memC :=
+  match goal with
+    | [ M : Mem |- _] =>  (* for all memories *)
+      match goal with
+      | [ H : mem_correct M |- _] => fail 1  (* already done *)
+      | [ |- _] =>  (* else *)
+         assert(mem_correct M) by (eapply BPreservation; eauto)
+      end
+    end.
+
+(*
+** {==================================================================
+** Equivalence big step - small step
+** ===================================================================
+*)
 
 Lemma stepBigstep : forall m e m' e' m'' e'',
     mem_correct m ->
@@ -247,16 +272,125 @@ Proof.
 Qed.
 
 
-(* Propagate 'mem_correct' to all memories *)
-Ltac memC :=
-  match goal with
-    | [ M : Mem |- _] =>  (* for all memories *)
-      match goal with
-      | [ H : mem_correct M |- _] => fail 1  (* already done *)
-      | [ |- _] =>  (* else *)
-         assert(mem_correct M) by (eapply BPreservation; eauto)
-      end
-    end.
+Ltac finishmExp :=
+  intros m e m' e' Hmt;
+  remember (Some e') as E' eqn:Heq;
+  generalize dependent e';
+  induction Hmt; intros ? Heq; inversion Heq; subst;
+  eauto using step,multistep.
+
+
+Lemma mPlus1 : forall e2 m e m' e',
+    m / e -->* m' / e' ->  m / IREPlus e e2 -->* m' / IREPlus e' e2.
+Proof. intros e2; finishmExp. Qed.
+
+Lemma mPlus2 : forall e1, Value e1 -> forall m e m' e',
+    m / e -->* m' / e' ->  m / IREPlus e1 e -->* m' / IREPlus e1 e'.
+Proof. intros e1 HV; finishmExp. Qed.
+
+Lemma mGet1 : forall e2 m e m' e',
+    m / e -->* m' / e' ->  m / IREGet e e2 -->* m' / IREGet e' e2.
+Proof. intros e2; finishmExp. Qed.
+
+Lemma mGet2 : forall e1, Value e1 -> forall m e m' e',
+    m / e -->* m' / e' ->  m / IREGet e1 e -->* m' / IREGet e1 e'.
+Proof. intros e1 HV; finishmExp. Qed.
+
+Lemma mSet1 : forall e2 e3 m e m' e',
+    m / e -->* m' / e' ->  m / IRESet e e2 e3 -->* m' / IRESet e' e2 e3.
+Proof. intros e2 e3; finishmExp. Qed.
+
+Lemma mSet2 : forall e1, Value e1 -> forall e3 m e m' e',
+    m / e -->* m' / e' ->  m / IRESet e1 e e3 -->* m' / IRESet e1 e' e3.
+Proof. intros e1 HV e3; finishmExp. Qed.
+
+Lemma mSet3 : forall e1 e2, Value e1 -> Value e2 -> forall m e m' e',
+    m / e -->* m' / e' ->  m / IRESet e1 e2 e -->* m' / IRESet e1 e2 e'.
+Proof. intros e1 e2 HV1 HV2; finishmExp. Qed.
+
+Lemma mLet1 : forall var t body m e m' e',
+    m / e -->* m' / e' ->
+    m / IRELet var t e body -->* m' / IRELet var t e' body.
+Proof. intros var t body; finishmExp. Qed.
+
+Lemma mFunapp1 : forall e2 m e m' e',
+    m / e -->* m' / e' ->  m / IREFunApp e e2 -->* m' / IREFunApp e' e2.
+Proof. intros e2; finishmExp. Qed.
+
+Lemma mFunapp2 : forall e1, Value e1 -> forall m e m' e',
+    m / e -->* m' / e' ->  m / IREFunApp e1 e -->* m' / IREFunApp e1 e'.
+Proof. intros e1 HV; finishmExp. Qed.
+
+Lemma mBox1 : forall t m e m' e',
+    m / e -->* m' / e' ->  m / IREBox t e -->* m' / IREBox t e'.
+Proof.
+  intros t; finishmExp. Qed.
+
+Lemma mUnbox1 : forall t m e m' e',
+    m / e -->* m' / e' ->  m / IREUnbox t e -->* m' / IREUnbox t e'.
+Proof. intros t; finishmExp. Qed.
+
+
+Theorem bigSmall : forall m e t m' e',
+    mem_correct m ->
+    MEmpty |= e : t ->
+    m / e ==> m' / e' ->
+    m / e -->* m' / e'.
+Proof.
+  intros m e t m' e' HM ? HSt.
+  remember (Some e') as E'.
+  generalize dependent e'.
+  generalize dependent t.
+  induction HSt; intros ? HTy ? Heq; inversion Heq; clear Heq; subst;
+  inversion HTy; subst;
+  repeat memC;
+  repeat match goal with
+    [ IH: mem_correct ?M  -> _ -> IRTyping _ ?E _ -> _,
+      HM: mem_correct ?M,
+      HT: IRTyping _ ?E _ |- _] =>
+        specialize (IH HM _ HT _ eq_refl)
+    end;
+    eauto using multistep.
+  - eauto 6 using mPlus1, mPlus2, Value, multistep1, step, multiRefl.
+  - eauto using multistep1, step.
+  - eauto 8 using mGet1, mGet2, Value, multistep1, step, multiRefl,
+                  BstepValue.
+  - eauto 12 using mSet1, mSet2, mSet3,  Value, multistep1, step, multiRefl,
+                  BstepValue.
+  - eapply multiRefl.
+    * eauto using mLet1.
+    * eapply multiRefl.
+      ** eauto using multistep1, StLet, BstepValue.
+      ** eauto using subst_typing, BstepValue, BstepTy.
+  -
+
+(*  - eapply multiRefl.
+    + eauto using mLambapp1.
+    + eapply multiRefl.
+      ** eauto using mLambapp2, Value.
+      ** eapply multiRefl.
+         *** eauto using multistep1, StLambapp, Value, BstepValue.
+         *** eapply IHHSt3; eauto.
+             eapply subst_typing.
+             2: { eapply BPreservation; eauto. }
+             assert (HX : MEmpty |= IRELamb var t body : ETLamb t1 t0).
+             { eapply BPreservation; eauto. }
+             inversion HX; subst.
+             eassumption.
+
+  - eapply multiRefl.
+    + eauto using mFunapp1.
+    + eapply multiRefl.
+      ** eauto using mFunapp2, Value.
+      ** eapply multiRefl.
+         *** eauto using multistep1, StFunapp, Value, BstepValue.
+         ***
+    +
+  -  *)
+Admitted.
+
+
+(* }================================================================== *)
 
 
 Theorem bigDyn : forall e t m e' m',
@@ -288,22 +422,16 @@ Proof.
     end; eauto using bigStep.
   - rewrite dynQuery. eauto using bigStep.
   - rewrite DynIndex. eauto using bigStep.
-  - apply (BStLambapp _ _ (dynMem m') var IRTStar (dyn body) _
-                          (dynMem m'') (dyn v2)); eauto.
+  - eapply BStLet; eauto. rewrite dynSubst.
+    eapply IHHB2; eauto.
+    eapply subst_typing; eauto. eauto using BstepTy.
+  - eapply BStFunapp; eauto.
+    + eapply BStUnbox. eauto.
     + rewrite dynSubst. eapply IHHB3; eauto.
-      assert (MEmpty |= IRELamb var t body : ETLamb t1 t0).
+      eapply subst_typing; eauto using BstepTy.
+      assert (HTyF: MEmpty |= IREFun var body : TgFun).
       { eapply BPreservation; eauto. }
-      eapply subst_typing; inversion H2; eauto.
-      eapply BPreservation; eauto.
-  - eapply (BStFunapp _ _ (dynMem m') var (dyn body) _ (dynMem m'')
-            (dyn v2)); eauto using bigStep.
-    + rewrite dynSubst. eapply IHHB3; eauto.
-      assert (HTF: MEmpty |= IREFun (IRELamb var IRTStar body) : TgFun).
-      { eapply BPreservation; eauto. }
-      inversion HTF; subst.
-      eapply subst_typing.
-      * inversion H5; eauto.
-      * eapply BPreservation; eauto.
+      inversion HTyF; subst. eauto.
 Qed.
 
 
